Phi_Semantics/PhiSem_Mem_C_MI.thy
@@ -18,11 +18,12 @@ proc calloc:
   requires \<open>\<p>\<a>\<r>\<a>\<m> T\<close>
   input \<open>n \<Ztypecolon> \<v>\<a>\<l> \<nat>(\<s>\<i>\<z>\<e>_\<t>)\<close>
   requires \<open>Semantic_Zero_Val TY T z\<close>
+  premises \<open>TY \<noteq> \<p>\<o>\<i>\<s>\<o>\<n>\<close>
   output \<open>replicate n z \<Ztypecolon> \<m>\<e>\<m>[addr] (\<m>\<e>\<m>-\<c>\<o>\<e>\<r>\<c>\<e> (Array n T))\<heavy_comma> addr \<Ztypecolon> \<v>\<a>\<l> TypedPtr (\<a>\<r>\<r>\<a>\<y>[n] TY)
           \<s>\<u>\<b>\<j> addr. memaddr.index addr = 0\<close>
   including Semantic_Zero_Val_EIF_brute
 \<medium_left_bracket>
-  note list_all2_conv_all_nth[simp] ;;
+  note list_all2_conv_all_nth[simp] \<semicolon>
 
   semantic_local_value($n) \<open>\<i>\<n>\<t>(\<s>\<i>\<z>\<e>_\<t>)\<close>
   semantic_assert \<open>Zero TY \<noteq> None\<close>
